finished remdups impl

SepLogicTime/Rev_Impl.thy
@@ -2,23 +2,24 @@ theory Rev_Impl
 imports SepAuto Asymptotics_Recurrences
 begin
 
-fun rev_fun :: "'a list \<Rightarrow> 'a list \<Rightarrow> nat \<Rightarrow> 'a list" where
-  "rev_fun xs ys 0 = ys"
-| "rev_fun xs ys (Suc n) = (let ys' = rev_fun xs ys n 
+fun rev'_fun :: "'a list \<Rightarrow> 'a list \<Rightarrow> nat \<Rightarrow> 'a list" where
+  "rev'_fun xs ys 0 = ys"
+| "rev'_fun xs ys (Suc n) = (let ys' = rev'_fun xs ys n 
                               in 
                                 ys'[n:=(xs!(length xs - Suc n))])"
-setup {* fold add_rewrite_rule @{thms rev_fun.simps} *}
+setup {* fold add_rewrite_rule @{thms rev'_fun.simps} *}
 
-lemma length_rev_fun[rewrite]: "length xs = length ys \<Longrightarrow> n\<le>length xs \<Longrightarrow> length (rev_fun xs ys n) = length ys"
-  apply(induct n) by auto
+lemma length_rev'_fun[rewrite]: "length xs = length ys \<Longrightarrow> n\<le>length xs \<Longrightarrow> length (rev'_fun xs ys n) = length ys"
+  by(induct n, auto) 
 
-lemma rev_fun_rev_aux: "length xs = length ys \<Longrightarrow> n \<le> length xs \<Longrightarrow> \<forall>i<n. rev_fun xs ys n ! i = rev xs ! i"
-  apply(induct n)
-  apply (auto) subgoal for n i by(cases "i=n", simp_all add: length_rev_fun rev_nth) done
+setup {* add_rewrite_rule @{thm rev_nth} *} 
 
-lemma rev_fun_correct[rewrite]: "length xs = length ys \<Longrightarrow> rev_fun xs ys (length xs) = rev xs"
-  apply(simp add: list_eq_iff_nth_eq length_rev_fun)
-  using rev_fun_rev_aux[where n="length xs"] by force
+lemma rev'_fun_rev_aux: "length xs = length ys \<Longrightarrow> n \<le> length xs \<Longrightarrow> 
+    i < n  \<Longrightarrow> rev'_fun xs ys n ! i = rev xs ! i"
+@proof @induct n arbitrary i @qed
+
+lemma rev'_fun_correct[rewrite]: "length xs = length ys \<Longrightarrow> rev'_fun xs ys (length ys) = rev xs"
+  by(auto simp add: rev'_fun_rev_aux list_eq_iff_nth_eq length_rev'_fun) 
 
 fun rev_impl' :: "('a::heap) array \<Rightarrow> 'a array \<Rightarrow> nat \<Rightarrow> unit Heap"  where 
   "rev_impl' p q 0 = return ()"
@@ -30,24 +31,28 @@ fun rev_impl' :: "('a::heap) array \<Rightarrow> 'a array \<Rightarrow> nat \<Ri
         return ()
       }"
 
-fun rev_impl'_time :: "nat \<Rightarrow> nat" where
-  "rev_impl'_time 0 = 1"
-| "rev_impl'_time (Suc n) = rev_impl'_time n + 4"
-setup {* fold add_rewrite_rule @{thms rev_impl'_time.simps} *}
+fun rev'_time :: "nat \<Rightarrow> nat" where
+  "rev'_time 0 = 1"
+| "rev'_time (Suc n) = rev'_time n + 4"
+setup {* fold add_rewrite_rule @{thms rev'_time.simps} *}
 
-lemma rev_impl'_time_closed: "rev_impl'_time n = (if n=0 then 1 else 1 + n*4)" 
+lemma rev'_time_closed: "rev'_time n = 1 + n*4" 
   by(induct n, auto)
 
-lemma rev_impl'_time_bound[asym_bound]: "rev_impl'_time \<in> \<Theta>(\<lambda>n. n)"
+lemma "rev'_time \<in> \<Theta>(\<lambda>n. n)"
+  unfolding rev'_time_closed by auto2
+
+lemma rev'_time_bound[asym_bound]: "rev'_time \<in> \<Theta>(\<lambda>n. n)"
   by(rule bigTheta_linear_recurrence_const[where g="\<lambda>_.4" and N=3], auto)
 
-lemma rev_impl'_rule'[hoare_triple]:
+lemma rev'_rule[hoare_triple]:
     "length xs = length ys \<Longrightarrow> n \<le> length xs \<Longrightarrow> 
-          <p \<mapsto>\<^sub>a xs * q \<mapsto>\<^sub>a ys * $(rev_impl'_time n)>
+          <p \<mapsto>\<^sub>a xs * q \<mapsto>\<^sub>a ys * $(rev'_time n)>
             rev_impl' p q n
-          <%_. p \<mapsto>\<^sub>a xs * q \<mapsto>\<^sub>a rev_fun xs ys n>\<^sub>t"
-@proof @fun_induct "rev_fun xs ys n" @qed
- 
+          <%_. p \<mapsto>\<^sub>a xs * q \<mapsto>\<^sub>a rev'_fun xs ys n>\<^sub>t"
+@proof @fun_induct "rev'_fun xs ys n" @qed
+
+
 definition rev_impl where
   "rev_impl p = do {
       len \<leftarrow> Array.len p;
@@ -56,22 +61,22 @@ definition rev_impl where
       return q
     }"
 
-definition rev_impl_time :: "nat \<Rightarrow> nat" where [rewrite]:
-  "rev_impl_time n = n + rev_impl'_time n + 3"
+definition rev_time :: "nat \<Rightarrow> nat" where [rewrite]:
+  "rev_time n = n + rev'_time n + 3"
 
-lemma rev_impl_time_mono: "x\<le>y \<Longrightarrow> rev_impl_time x \<le> rev_impl_time y"
-  unfolding rev_impl_time_def rev_impl'_time_closed by auto   
+lemma rev_impl_time_mono: "x\<le>y \<Longrightarrow> rev_time x \<le> rev_time y"
+  unfolding rev_time_def rev'_time_closed by auto   
 
-lemma rev_impl_time_bound[asym_bound]: "rev_impl_time \<in> \<Theta>(\<lambda>n. n)"
-  unfolding rev_impl_time_def by auto2
+lemma rev_impl_time_bound[asym_bound]: "rev_time \<in> \<Theta>(\<lambda>n. n)"
+  unfolding rev_time_def by auto2
 
 lemma rev_impl_rule[hoare_triple]:
     "length xs = length ys \<Longrightarrow>
-          <p \<mapsto>\<^sub>a xs * $(rev_impl_time (length xs))>
+          <p \<mapsto>\<^sub>a xs * $(rev_time (length xs))>
             rev_impl p
           <%r. p \<mapsto>\<^sub>a xs * r \<mapsto>\<^sub>a rev xs>\<^sub>t"
   by auto2
 
-setup {* del_prfstep_thm @{thm rev_impl_time_def} *} 
+setup {* del_prfstep_thm @{thm rev_time_def} *} 
 
 end
